Code cleanup

src/HList.v
@@ -1,12 +1,13 @@
 Set Implicit Arguments.
 Unset Strict Implicit.
 
+Require Import Coq.Lists.List.
+Import ListNotations.
 Require Import Omega.
+
 Require Import CrossCrypto.FrapTactics.
 Require Import CrossCrypto.ListUtil.
 Require Import CrossCrypto.Tuple.
-Require Import Coq.Lists.List.
-Import ListNotations.
 
 Inductive hlist A (f : A -> Type) : list A -> Type :=
 | hnil : hlist f []
@@ -15,7 +16,8 @@ Inductive hlist A (f : A -> Type) : list A -> Type :=
 Notation " h[] " := (hnil _).
 Infix "h::" := hcons (at level 60, right associativity).
 
-Definition hhead A f (l : list A) (hl : hlist f l) (H : l <> []) : f (head_with_proof H).
+Definition hhead A f (l : list A) (hl : hlist f l) (H : l <> []) :
+  f (head_with_proof H).
   inversion hl.
   congruence.
   subst l.
@@ -30,13 +32,15 @@ Definition htail A f (l : list A) (hl : hlist f l) : hlist f (tl l).
   exact X0.
 Defined.
 
-Fixpoint list2hlist T (A : T) (f : T -> Type) (fl : list (f A)) : hlist f (repeat A (length fl)).
+Fixpoint list2hlist T (A : T) (f : T -> Type) (fl : list (f A)) :
+  hlist f (repeat A (length fl)).
   cases fl.
   exact (h[]).
   exact (f0 h:: list2hlist T A f fl).
 Defined.
 
-Fixpoint hlist2list A (f : A -> Type) l (hl : hlist f l) (x : A) (H : exists n , l = repeat x n) : list (f x).
+Fixpoint hlist2list A (f : A -> Type) l (hl : hlist f l) (x : A)
+         (H : exists n , l = repeat x n) : list (f x).
   cases hl.
   exact [].
   refine (_ :: hlist2list A f l hl x _).
@@ -67,12 +71,16 @@ Fixpoint tuple2hlist A (T : A) P n (t : tuple (P T) n)
   induction t; constructor; assumption.
 Defined.
 
-Lemma hlist2list_len : forall A (f : A -> Type) (l : list A) (hl : hlist f l) (x : A) (P : exists n, l = repeat x n), length (hlist2list hl P) = length l.
+Lemma hlist2list_len :
+  forall A (f : A -> Type) (l : list A) (hl : hlist f l) (x : A)
+         (P : exists n, l = repeat x n),
+    length (hlist2list hl P) = length l.
 Proof.
   induct hl; simplify; equality.
 Qed.
 
-Definition hlist2tuple (A : Type) (f : A -> Type) (l : list A) (hl : hlist f l) (x : A) n (P : l = repeat x n) : tuple (f x) n.
+Definition hlist2tuple (A : Type) (f : A -> Type) (l : list A)
+           (hl : hlist f l) (x : A) n (P : l = repeat x n) : tuple (f x) n.
   assert (exists n0 : nat, l = repeat x n0).
   exists n.
   assumption.
@@ -81,13 +89,12 @@ Definition hlist2tuple (A : Type) (f : A -> Type) (l : list A) (hl : hlist f l) 
   apply hlist2list_len.
   rewrite H0.
   rewrite P.
-  Locate repeat.
   symmetry.
   apply repeat_length.
   rewrite H0.
   exact (list2tuple (hlist2list hl H)).
 Defined.
-        
+
 Definition hmap A (f : A -> Type) B (g : B -> Type)
            (F : A -> B) (F' : forall a, f a -> g (F a))
            (l : list A) (h : hlist f l) : hlist g (map F l).
@@ -102,4 +109,3 @@ Definition hmap' A (f : A -> Type) (g : A -> Type)
   clear f g F' h.
   induction l as [| x xs IHl]; [| simpl; rewrite IHl]; reflexivity.
 Defined.
-
