src/Models.v
@@ -1,268 +1,311 @@
 Set Implicit Arguments.
 
-Require Import CrossCrypto.FirstOrder.
 Require Import Coq.Lists.List.
 Import ListNotations.
 
-Section Models.
-
-  (* Finite bound on the number of random values you and the attacker will need. *)
-  Context (rand_bound : nat).
-  Context (arand_bound : nat).
-
-Section SymbolicModel.
-
-  Inductive SymbolicSort :=
-  | Message : SymbolicSort
-  | Bool : SymbolicSort.
-
-  Inductive SymbolicFunc : list SymbolicSort -> SymbolicSort -> Type :=
-  | STrue : SymbolicFunc [] Bool
-  | SFalse : SymbolicFunc [] Bool
-  | IfThenElse : SymbolicFunc (Bool :: Message :: Message :: []) Message
-  | EmptyMsg : SymbolicFunc [] Message
-  | Eq : SymbolicFunc (Message :: Message :: []) Bool
-  | EqL : SymbolicFunc (Message :: Message :: []) Bool
-
-  | Name : forall (n : nat), n < rand_bound -> (SymbolicFunc [] Message)
-  | AName : forall (n : nat), n < arand_bound -> (SymbolicFunc [] Message)
-  | Handle : forall (n : nat) (dom : list SymbolicSort) (cod : SymbolicSort), SymbolicFunc dom cod.
-
-  (* Indistinguishability is defined on both messages and booleans *)
-  Inductive SymbolicPredicate : list SymbolicSort -> Type :=
-    | Indist : forall (l1 l2 : list SymbolicSort) (H: length l1 = length l2), SymbolicPredicate (l1 ++ l2).
-
-End SymbolicModel.
-
-Require Import WC_PolyTime.
-Require Import Admissibility.
-Require Import Asymptotic.
-Require Import FCF.
-
 Require Import CrossCrypto.CompUtil.
+Require Import CrossCrypto.FirstOrder.
 Require Import CrossCrypto.FrapTactics.
 Require Import CrossCrypto.HList.
 Require Import CrossCrypto.Tuple.
 
-Section CompInterp.
+Section Models.
 
-  Context `{function_cost_model}.
-  (* TODO: actual definition of reasonable *)
-  Definition reasonable (cost : FunctionCostModel) := True.
+  (* Finite bound on the number of random values you and the attacker
+     will need. *)
+  Context (rand_bound : nat).
+  Context (arand_bound : nat).
 
-  Context `{reasonable cost}.
+  Section SymbolicModel.
 
-  Definition message := {n : nat & Bvector n}.
-  Definition rands (eta : nat) := tuple (Bvector eta) rand_bound.
-  Definition arands (eta : nat) := tuple (Bvector eta) arand_bound.
-  Definition comp (S : Set) := forall (eta : nat), rands eta -> arands eta -> Comp S.
+    Inductive SymbolicSort :=
+    | Message : SymbolicSort
+    | Bool : SymbolicSort.
 
-  Definition curry_rands_func T eta (c : rands eta -> arands eta -> Comp T) : tuple (Bvector eta) (rand_bound + arand_bound) -> Comp T.
-    intros.
-    remember (tskipn H0 rand_bound) as arand.
-    assert (rand_bound + arand_bound - rand_bound = arand_bound).
-    linear_arithmetic.
-    clear Heqarand.
-    rewrite H1 in arand.
-    refine (c (tfirstn H0 _) arand).
-    linear_arithmetic.
-  Defined.
+    Inductive SymbolicFunc : list SymbolicSort -> SymbolicSort -> Type :=
+    | STrue : SymbolicFunc [] Bool
+    | SFalse : SymbolicFunc [] Bool
+    | IfThenElse : SymbolicFunc (Bool :: Message :: Message :: []) Message
+    | EmptyMsg : SymbolicFunc [] Message
+    | Eq : SymbolicFunc (Message :: Message :: []) Bool
+    | EqL : SymbolicFunc (Message :: Message :: []) Bool
 
-  Definition bind_rands T eta (c : rands eta -> arands eta -> Comp T) : Comp T :=
-    bind_tuple (curry_rands_func c).
+    | Name : forall (n : nat), n < rand_bound -> (SymbolicFunc [] Message)
+    | AName : forall (n : nat), n < arand_bound -> (SymbolicFunc [] Message)
+    | Handle : forall (n : nat) (dom : list SymbolicSort) (cod : SymbolicSort),
+        SymbolicFunc dom cod.
 
-  Lemma message_eq_dec : forall (m n : message), {m = n} + {m <> n}.
-    intros.
-    destruct m; destruct n.
-    cases (x ==n x0).
-    subst x.
-    cases (Bvector_eq_dec b b0).
-    subst b.
-    left.
-    congruence.
-    right.
-    intuition.
-    right.
-    congruence.
-  Defined.
+    (* Indistinguishability is defined on both messages and booleans *)
+    Inductive SymbolicPredicate : list SymbolicSort -> Type :=
+    | Indist : forall (l1 l2 : list SymbolicSort) (H: length l1 = length l2),
+        SymbolicPredicate (l1 ++ l2).
 
-  (* TODO : Probably shouldn't need to explicitly set and unset here *)
-  Unset Implicit Arguments.
-  Record MessageComp :=
-    mkMessageComp {
-        message_comp : comp message;
-        message_poly : admissible_oc cost (fun _ => unit) (fun _ => unit) (fun _ => message) (fun (eta : nat) =>
-                                                                                                OC_Ret unit unit (bind_rands (message_comp eta)))
-      }.
+  End SymbolicModel.
 
-  Record BoolComp :=
-    mkBoolComp {
-        bool_comp : comp bool;
-        bool_poly : admissible_oc cost (fun _ => unit) (fun _ => unit) (fun _ => bool) (fun (eta : nat) => OC_Ret unit unit (bind_rands (bool_comp eta)))
-      }.
-  Set Implicit Arguments.
+  Require Import Admissibility.
+  Require Import Asymptotic.
+  Require Import FCF.
+  Require Import WC_PolyTime.
 
-  Definition CompDomain (s : SymbolicSort) : Type :=
-    match s with
-    | Message => MessageComp
-    | Bool => BoolComp
-    end.
+  Section CompInterp.
 
-  Ltac trivial_polynomial :=
-    unfold polynomial; exists 0%nat; exists 0%nat; exists 0%nat; unfold expnat; simpl; intros; omega.
+    Context `{function_cost_model}.
+    (* TODO: actual definition of reasonable *)
+    Definition reasonable (cost : FunctionCostModel) := True.
 
-  Lemma constant_polytime : forall T (eq : eq_dec T) (b : T),
-      admissible_oc cost (fun _ => unit) (fun _ => unit) (fun _ => T) (fun (eta : nat) => OC_Ret unit unit (bind_rands (fun _ : rands eta => fun _ : arands eta => Ret eq b))).
-  Admitted.
+    Context `{reasonable cost}.
 
-  Definition constant_boolcomp (b : bool) : BoolComp :=
-    mkBoolComp (fun _ _ _ => Ret bool_dec b) (constant_polytime bool_dec b).
+    Definition message := {n : nat & Bvector n}.
+    Definition rands (eta : nat) := tuple (Bvector eta) rand_bound.
+    Definition arands (eta : nat) := tuple (Bvector eta) arand_bound.
+    Definition comp (S : Set) := forall (eta : nat),
+        rands eta -> arands eta -> Comp S.
 
-  Definition constant_messagecomp (m : message) : MessageComp :=
-    mkMessageComp (fun _ _ _ => Ret message_eq_dec m) (constant_polytime message_eq_dec m).
+    Definition curry_rands_func T eta (c : rands eta -> arands eta -> Comp T) :
+      tuple (Bvector eta) (rand_bound + arand_bound) -> Comp T.
+      intros.
+      remember (tskipn H0 rand_bound) as arand.
+      assert (rand_bound + arand_bound - rand_bound = arand_bound).
+      linear_arithmetic.
+      clear Heqarand.
+      rewrite H1 in arand.
+      refine (c (tfirstn H0 _) arand).
+      linear_arithmetic.
+    Defined.
 
-  Definition if_then_else_comp (b : comp bool) (m1 m2 : comp message) : comp message :=
-    fun (eta : nat) =>
-      fun (r : rands eta) =>
-        fun (ar : arands eta) =>
-      b' <-$ (b eta r ar);
-        (if b' then m1 else m2) eta r ar.
+    Definition bind_rands T eta (c : rands eta -> arands eta -> Comp T) :
+      Comp T :=
+      bind_tuple (curry_rands_func c).
 
-  Definition if_then_else_poly: forall (b : BoolComp) (m1 m2 : MessageComp),
-      admissible_oc cost (fun _ : nat => unit) (fun _ : nat => unit) (fun _ : nat => message)
-                    (fun (eta : nat) => $ (bind_rands ((if_then_else_comp (bool_comp b) (message_comp m1) (message_comp m2)) eta))).
-  Admitted.
+    Lemma message_eq_dec : forall (m n : message), {m = n} + {m <> n}.
+      intros.
+      destruct m; destruct n.
+      cases (x ==n x0).
+      subst x.
+      cases (Bvector_eq_dec b b0).
+      subst b.
+      left.
+      congruence.
+      right.
+      intuition.
+      right.
+      congruence.
+    Defined.
 
-  Definition if_then_else_messagecomp (b : BoolComp) (m1 m2 : MessageComp) : MessageComp :=
-    mkMessageComp (if_then_else_comp b.(bool_comp) m1.(message_comp) m2.(message_comp)) (if_then_else_poly b m1 m2).
+    (* TODO : Probably shouldn't need to explicitly set and unset here *)
+    Unset Implicit Arguments.
+    Record MessageComp :=
+      mkMessageComp {
+          message_comp : comp message;
+          message_poly :
+            admissible_oc cost
+                          (fun _ => unit)
+                          (fun _ => unit)
+                          (fun _ => message)
+                          (fun (eta : nat) =>
+                             OC_Ret unit unit (bind_rands (message_comp eta)))
+        }.
 
-  Definition message_eq (m1 m2 : message) : bool.
-    cases (message_eq_dec m1 m2).
-    exact true.
-    exact false.
-  Defined.
+    Record BoolComp :=
+      mkBoolComp {
+          bool_comp : comp bool;
+          bool_poly :
+            admissible_oc cost
+                          (fun _ => unit)
+                          (fun _ => unit)
+                          (fun _ => bool)
+                          (fun (eta : nat) =>
+                             OC_Ret unit unit (bind_rands (bool_comp eta)))
+        }.
+    Set Implicit Arguments.
 
-  Definition EqDec_message : EqDec message.
-    refine (Build_EqDec _ _).
-    intros.
-    cases (message_eq_dec x y).
-    instantiate (1 := fun m1 m2 => message_eq m1 m2).
-    split; simplify; try assumption.
-    unfold message_eq.
-    cases (message_eq_dec x y).
-    trivial.
-    contradiction.
-    split; simplify; try assumption.
-    unfold message_eq in H0.
-    cases (message_eq_dec x y); try equality.
-    equality.
-  Defined.
+    Definition CompDomain (s : SymbolicSort) : Type :=
+      match s with
+      | Message => MessageComp
+      | Bool => BoolComp
+      end.
 
-  Definition eq_comp (m1 m2 : comp message) : comp bool.
-    refine (fun (eta : nat) =>
-              fun (r : rands eta) =>
-                fun (ar : arands eta) =>
-              m1' <-$ m1 eta r ar;
-              m2' <-$ m2 eta r ar;
-              ret (m1' ?= m2')).
-    apply EqDec_message.
-  Defined.
+    Ltac trivial_polynomial :=
+      unfold polynomial; exists 0%nat; exists 0%nat; exists 0%nat;
+      unfold expnat; simpl; intros; omega.
 
-  Definition eq_poly: forall (m1 m2 : MessageComp),
-      admissible_oc cost (fun _ : nat => unit) (fun _ : nat => unit) (fun _ : nat => bool)
-                    (fun eta : nat => $ (bind_rands ((eq_comp (message_comp m1) (message_comp m2)) eta))).
-  Admitted.
+    Lemma constant_polytime : forall T (eq : eq_dec T) (b : T),
+        admissible_oc cost (fun _ => unit)
+                      (fun _ => unit)
+                      (fun _ => T)
+                      (fun (eta : nat) =>
+                         OC_Ret unit unit
+                                (bind_rands
+                                   (fun _ : rands eta =>
+                                      fun _ : arands eta => Ret eq b))).
+    Admitted.
 
-  Definition eq_boolcomp (m1 m2 : MessageComp) : BoolComp :=
-    mkBoolComp (eq_comp m1.(message_comp) m2.(message_comp)) (eq_poly m1 m2).
+    Definition constant_boolcomp (b : bool) : BoolComp :=
+      mkBoolComp (fun _ _ _ => Ret bool_dec b) (constant_polytime bool_dec b).
 
-  Definition eql_comp (m1 m2 : comp message) : comp bool.
-    refine (fun (eta : nat) =>
-              fun (r : rands eta) =>
-                fun (ar : arands eta) =>
-              m1' <-$ m1 eta r ar;
-              m2' <-$ m2 eta r ar;
-              ret _).
-    destruct m1'; destruct m2'.
-    exact (x ?= x0).
-  Defined.
+    Definition constant_messagecomp (m : message) : MessageComp :=
+      mkMessageComp (fun _ _ _ => Ret message_eq_dec m)
+                    (constant_polytime message_eq_dec m).
 
-  Definition eql_poly: forall (m1 m2 : MessageComp),
-      admissible_oc cost (fun _ : nat => unit) (fun _ : nat => unit) (fun _ : nat => bool)
-                    (fun eta : nat => $ (bind_rands ((eql_comp (message_comp m1) (message_comp m2)) eta))).
-  Admitted.
+    Definition if_then_else_comp (b : comp bool) (m1 m2 : comp message) :
+      comp message :=
+      fun (eta : nat) =>
+        fun (r : rands eta) =>
+          fun (ar : arands eta) =>
+            b' <-$ (b eta r ar);
+              (if b' then m1 else m2) eta r ar.
 
-  Definition eql_boolcomp (m1 m2 : MessageComp) : BoolComp :=
-    mkBoolComp (eql_comp m1.(message_comp) m2.(message_comp)) (eql_poly m1 m2).
+    Definition if_then_else_poly: forall (b : BoolComp) (m1 m2 : MessageComp),
+        admissible_oc cost
+                      (fun _ : nat => unit)
+                      (fun _ : nat => unit)
+                      (fun _ : nat => message)
+                      (fun (eta : nat) => $ (bind_rands
+                                               ((if_then_else_comp
+                                                   (bool_comp b)
+                                                   (message_comp m1)
+                                                   (message_comp m2)) eta))).
+    Admitted.
 
-  Definition name_comp (n : nat) (H' : n < rand_bound) : comp message.
-    refine (fun (eta : nat) =>
-              fun (r : rands eta) =>
-                fun (ar : arands eta) =>
-                ret (existT Bvector eta (tnth r H'))).
-    exact EqDec_message.
-  Defined.
+    Definition if_then_else_messagecomp (b : BoolComp) (m1 m2 : MessageComp) :
+      MessageComp :=
+      mkMessageComp (if_then_else_comp _ _ _)
+                    (if_then_else_poly b m1 m2).
 
-  Definition name_poly: forall (n : nat) (H' : n < rand_bound),
-      admissible_oc cost (fun _ : nat => unit) (fun _ : nat => unit) (fun _ : nat => message)
-                    (fun eta : nat => $ (bind_rands ((name_comp H') eta))).
-  Admitted.
+    Definition message_eq (m1 m2 : message) : bool.
+      cases (message_eq_dec m1 m2).
+      exact true.
+      exact false.
+    Defined.
 
-  Definition name_messagecomp (n : nat) (H' : n < rand_bound) : MessageComp :=
-    mkMessageComp (name_comp H') (name_poly H').
+    Definition EqDec_message : EqDec message.
+      refine (Build_EqDec message_eq _).
+      unfold message_eq.
+      intros x y.
+      destruct (message_eq_dec x y); intuition.
+    Defined.
 
-  (* Axiom TODO : forall {T : Type}, T. *)
+    Definition eq_comp (m1 m2 : comp message) : comp bool.
+      refine (fun (eta : nat) =>
+                fun (r : rands eta) =>
+                  fun (ar : arands eta) =>
+                    m1' <-$ m1 eta r ar;
+                    m2' <-$ m2 eta r ar;
+                    ret (m1' ?= m2')).
+      apply EqDec_message.
+    Defined.
 
-  (* Definition interp_handles := forall (n : nat) (dom : list SymbolicSort) (cod : SymbolicSort) (h : hlist CompDomain dom), CompDomain cod. *)
+    Definition eq_poly: forall (m1 m2 : MessageComp),
+        admissible_oc cost
+                      (fun _ : nat => unit)
+                      (fun _ : nat => unit)
+                      (fun _ : nat => bool)
+                      (fun eta : nat => $ (bind_rands
+                                             ((eq_comp
+                                                 (message_comp m1)
+                                                 (message_comp m2)) eta))).
+    Admitted.
 
-  (* Definition CompInterpFunc dom cod (s : SymbolicFunc dom cod) (h : hlist CompDomain dom) (ih : interp_handles) : (CompDomain cod). *)
-  (*   induction s. *)
-  (*   (* STrue *) *)
-  (*   - exact (constant_boolcomp true). *)
-  (*   (* SFalse *) *)
-  (*   - exact (constant_boolcomp false). *)
-  (*   (* IfThenElse *) *)
-  (*   - refine (if_then_else_messagecomp _ _ _). *)
-  (*     inversion h. *)
-  (*     exact X. *)
-  (*     inversion h. *)
-  (*     inversion X0. *)
-  (*     exact X1. *)
-  (*     inversion h. *)
-  (*     inversion X0. *)
-  (*     inversion X2. *)
-  (*     exact X3. *)
-  (*   (* EmptyMsg *) *)
-  (*   - exact (constant_messagecomp (existT Bvector 0 Bnil)%nat). *)
-  (*   (* Eq *) *)
-  (*   - refine (eq_boolcomp _ _). *)
-  (*     inversion h. *)
-  (*     exact X. *)
-  (*     inversion h. *)
-  (*     inversion X0. *)
-  (*     exact X1. *)
-  (*   (* EqL *) *)
-  (*   - refine (eql_boolcomp _ _). *)
-  (*     inversion h. *)
-  (*     exact X. *)
-  (*     inversion h. *)
-  (*     inversion X0. *)
-  (*     exact X1. *)
-  (*   (* Name *) *)
-  (*   - exact (name_messagecomp l). *)
-  (*   (* Handle *) *)
-  (*   - exact (ih n dom cod h). *)
-  (* Defined. *)
+    Definition eq_boolcomp (m1 m2 : MessageComp) : BoolComp :=
+      mkBoolComp (eq_comp _ _) (eq_poly m1 m2).
+
+    Definition eql_comp (m1 m2 : comp message) : comp bool.
+      refine (fun (eta : nat) =>
+                fun (r : rands eta) =>
+                  fun (ar : arands eta) =>
+                    m1' <-$ m1 eta r ar;
+                    m2' <-$ m2 eta r ar;
+                    ret _).
+      destruct m1'; destruct m2'.
+      exact (x ?= x0).
+    Defined.
+
+    Definition eql_poly: forall (m1 m2 : MessageComp),
+        admissible_oc cost
+                      (fun _ : nat => unit)
+                      (fun _ : nat => unit)
+                      (fun _ : nat => bool)
+                      (fun eta : nat => $ (bind_rands
+                                             ((eql_comp
+                                                 (message_comp m1)
+                                                 (message_comp m2)) eta))).
+    Admitted.
+
+    Definition eql_boolcomp (m1 m2 : MessageComp) : BoolComp :=
+      mkBoolComp (eql_comp _ _) (eql_poly m1 m2).
+
+    Definition name_comp (n : nat) (H' : n < rand_bound) : comp message.
+      refine (fun (eta : nat) =>
+                fun (r : rands eta) =>
+                  fun (ar : arands eta) =>
+                    ret (existT Bvector eta (tnth r H'))).
+      exact EqDec_message.
+    Defined.
+
+    Definition name_poly: forall (n : nat) (H' : n < rand_bound),
+        admissible_oc cost
+                      (fun _ : nat => unit)
+                      (fun _ : nat => unit)
+                      (fun _ : nat => message)
+                      (fun eta : nat => $ (bind_rands ((name_comp H') eta))).
+    Admitted.
+
+    Definition name_messagecomp (n : nat) (H' : n < rand_bound) :
+      MessageComp :=
+      mkMessageComp (name_comp H') (name_poly H').
+
+    (* Axiom TODO : forall {T : Type}, T. *)
+
+    (* Definition interp_handles := forall (n : nat) (dom : list SymbolicSort) (cod : SymbolicSort) (h : hlist CompDomain dom), CompDomain cod. *)
+
+    (* Definition CompInterpFunc dom cod (s : SymbolicFunc dom cod) (h : hlist CompDomain dom) (ih : interp_handles) : (CompDomain cod). *)
+    (*   induction s. *)
+    (*   (* STrue *) *)
+    (*   - exact (constant_boolcomp true). *)
+    (*   (* SFalse *) *)
+    (*   - exact (constant_boolcomp false). *)
+    (*   (* IfThenElse *) *)
+    (*   - refine (if_then_else_messagecomp _ _ _). *)
+    (*     inversion h. *)
+    (*     exact X. *)
+    (*     inversion h. *)
+    (*     inversion X0. *)
+    (*     exact X1. *)
+    (*     inversion h. *)
+    (*     inversion X0. *)
+    (*     inversion X2. *)
+    (*     exact X3. *)
+    (*   (* EmptyMsg *) *)
+    (*   - exact (constant_messagecomp (existT Bvector 0 Bnil)%nat). *)
+    (*   (* Eq *) *)
+    (*   - refine (eq_boolcomp _ _). *)
+    (*     inversion h. *)
+    (*     exact X. *)
+    (*     inversion h. *)
+    (*     inversion X0. *)
+    (*     exact X1. *)
+    (*   (* EqL *) *)
+    (*   - refine (eql_boolcomp _ _). *)
+    (*     inversion h. *)
+    (*     exact X. *)
+    (*     inversion h. *)
+    (*     inversion X0. *)
+    (*     exact X1. *)
+    (*   (* Name *) *)
+    (*   - exact (name_messagecomp l). *)
+    (*   (* Handle *) *)
+    (*   - exact (ih n dom cod h). *)
+    (* Defined. *)
 
 
-(* Definition indist_comp : bool. *)
-(* Definition indist dom (l1 l2 : hlist CompDomain dom) : Prop. *)
+    (* Definition indist_comp : bool. *)
+    (* Definition indist dom (l1 l2 : hlist CompDomain dom) : Prop. *)
 
-(* Definition CompInterpPredicate dom (s : SymbolicPredicate dom) (h : hlist CompDomain dom) : Prop. *)
-(*   induction s. *)
-(* About model. *)
-(* (* Definition CompModel := Model SymbolicSort SymbolicFunc SymbolicState *) *)
+    (* Definition CompInterpPredicate dom (s : SymbolicPredicate dom) (h : hlist CompDomain dom) : Prop. *)
+    (*   induction s. *)
+    (* About model. *)
+    (* (* Definition CompModel := Model SymbolicSort SymbolicFunc SymbolicState *) *)
 
-End CompInterp.
+  End CompInterp.
 
 End Models.
