src/CompUtil.v
@@ -9,19 +9,25 @@ Require Import CrossCrypto.FrapTactics.
 Require Import CrossCrypto.HList.
 Require Import CrossCrypto.Tuple.
 
-(* This is a weird way of doing things but I couldn't figure out a good workaround *)
+(* This is a weird way of doing things but I couldn't figure out a good
+   workaround *)
 Definition set2type (A : Set) : Type := A.
 
-Fixpoint bind_comps (comp_types: list Set) (h : hlist Comp comp_types) T (f : hlist set2type comp_types -> Comp T) {struct comp_types} : Comp T.
+Fixpoint bind_comps (comp_types : list Set) (h : hlist Comp comp_types) T
+         (f : hlist set2type comp_types -> Comp T) {struct comp_types} :
+  Comp T.
   cases comp_types.
   exact (f h[]).
-  refine (bind_comps comp_types (htail h) T (fun (f' : hlist set2type comp_types) => Bind _ (fun x => f (_ h:: f')))).
+  refine (bind_comps comp_types (htail h) T
+                     (fun (f' : hlist set2type comp_types) =>
+                        Bind _ (fun x => f (_ h:: f')))).
   refine (hhead h _).
   equality.
   exact x.
 Defined.
 
-Definition bind_tuple T {eta : nat} n (f : tuple (Bvector eta) n -> Comp T) : Comp T.
+Definition bind_tuple T {eta : nat} n
+           (f : tuple (Bvector eta) n -> Comp T) : Comp T.
   refine (bind_comps (list2hlist (repeat (Rnd eta) n)) _).
   refine (fun h => f (hlist2tuple h _ )).
   assert (length (repeat (Rnd eta) n) = n).
