src/ListUtil.v
@@ -1,9 +1,10 @@
 Set Implicit Arguments.
 
-Require Import Omega.
-Require Import CrossCrypto.FrapTactics.
 Require Import Coq.Lists.List.
 Import ListNotations.
+Require Import Omega.
+
+Require Import CrossCrypto.FrapTactics.
 
 Definition head_with_proof T (l : list T) (H : l <> []) : T.
   destruct l.
@@ -11,7 +12,9 @@ Definition head_with_proof T (l : list T) (H : l <> []) : T.
   exact t.
 Defined.
 
-Fixpoint nth_with_proof T (n:nat) (l:list T) (H : length(l) > n) {struct l} : T.
+Fixpoint nth_with_proof T (n:nat) (l:list T) {struct l} :
+  length(l) > n -> T.
+  intro H.
   FrapTactics.cases n; FrapTactics.cases l; FrapTactics.simplify; try omega.
   exact t.
   refine (nth_with_proof T n l _).
